Clean up Fix-Join theory (remove cruft, rename primed lemmas)

isa-launchbury/HOLCF-Fix-Join.thy
@@ -2,145 +2,61 @@ theory "HOLCF-Fix-Join"
   imports "HOLCF-Set" "HOLCF-Join" "HOLCF-Down-Closed"
 begin
 
-definition fix_join_compat' :: "'a::{Bounded_Nonempty_Meet_cpo,subpcpo_partition} \<Rightarrow> 'a set"
-  where "fix_join_compat' \<rho> = {x. compatible \<rho> x}"
+subsubsection {* A carrier set for fixed points of binary joins *}
 
-lemma fjc'_iff[iff]:
-  "x \<in> fix_join_compat' \<rho> \<longleftrightarrow> compatible \<rho> x"
-  unfolding fix_join_compat'_def by auto
+text {* @{term fix_join_compat} is a set in which the join operation is always defined, and can
+serve as carrier sets for the various HOLCF-Set operations. *}
 
-lemma subcpo_jfc': "subcpo (fix_join_compat' \<rho>)"
-  apply (rule subcpoI)
-  apply simp
-  apply (rule admD[OF compatible_adm2])
-  apply assumption+
-  done
+definition fix_join_compat where 
+  "fix_join_compat (\<rho>::'a::{Bounded_Nonempty_Meet_cpo,subpcpo_partition})  F = {\<rho>'. \<rho>' \<sqsubseteq> fix_on' (to_bot \<rho>) (\<lambda> \<rho>'. \<rho> \<squnion> F \<rho>')}"
 
-lemma compatible_to_bot: "compatible x y \<Longrightarrow> to_bot y = to_bot x"
-by (metis join_above1 join_above2 unrelated)
+lemma fjc_iff[iff]:
+  "\<rho>' \<in> fix_join_compat \<rho> F \<longleftrightarrow> \<rho>' \<sqsubseteq> fix_on' (to_bot \<rho>) (\<lambda> \<rho>'. \<rho> \<squnion> F \<rho>')"
+  unfolding fix_join_compat_def by auto
 
-lemma subpcpo_bot_jfc': "subpcpo_bot (fix_join_compat' \<rho>) (to_bot \<rho>)"
+lemma subcpo_fjc: "subcpo (fix_join_compat \<rho> F)"
+  unfolding fix_join_compat_def by (rule subcpo_cone_below)
+
+lemma subpcpo_fjc: "subpcpo (fix_join_compat \<rho> F)"
+  unfolding fix_join_compat_def by (rule subpcpo_cone_below)
+
+lemma subpcpo_bot_fjc: "subpcpo_bot (fix_join_compat \<rho> F) (to_bot \<rho>)"
   apply (rule subpcpo_botI)
-  apply (metis subcpo.cpo' subcpo_jfc')
-  apply (auto)
-  apply (metis below.r_refl compatibleI to_bot_minimal)
-  by (metis compatible_to_bot to_bot_minimal)
-
-lemma subpcpo_jfc': "subpcpo (fix_join_compat' \<rho>)"
-   by (rule subpcpo_bot_is_subpcpo[OF subpcpo_bot_jfc'])
-
-lemma bottom_of_jfc': "bottom_of (fix_join_compat' \<rho>) = to_bot \<rho>"
-  by (rule bottom_of_subpcpo_bot[OF subpcpo_bot_jfc'])
-
-lemma down_closed_jfc': "down_closed (fix_join_compat' \<rho>)"
-  apply (rule down_closedI)
-  unfolding fix_join_compat'_def
-  apply simp
-  by (rule compatible_down_closed2)
-
-lemma compat_jfc': "x \<in> fix_join_compat' \<rho> \<Longrightarrow> compatible \<rho> x"  by simp
-
-context
-  fixes \<rho> :: "'a::{Bounded_Nonempty_Meet_cpo,subpcpo_partition}"
-  fixes F :: "'a \<Rightarrow> 'a"
-  assumes "cont F"
-  assumes F_pres_compat: "\<And> x. compatible \<rho> x \<Longrightarrow> compatible \<rho> (F x)"
-begin
-
-  lemma compatible_F_jfc': "x \<in> fix_join_compat' \<rho> \<Longrightarrow> compatible \<rho> (F x)"
-    by (metis F_pres_compat compat_jfc')
-
-  lemma closed_jfc': "x \<in> (fix_join_compat' \<rho>) \<Longrightarrow> \<rho> \<squnion> F x \<in> (fix_join_compat' \<rho>)"
-    apply auto
-    by (metis "HOLCF-Join.join_above1" F_pres_compat below.r_refl compatibleI)
-
-  lemma closed_on_jfc': "closed_on (fix_join_compat' \<rho>) (\<lambda> x. \<rho> \<squnion> F x)"
-    by (rule closed_onI, rule closed_jfc')
-
-  lemma cont_on_jfc': "cont_on (fix_join_compat' \<rho>) (\<lambda> x. \<rho> \<squnion> F x)"
-  proof(rule subpcpo.cont_onI2[OF subpcpo_jfc'])
-  case goal1 show ?case
-    apply (rule monofun_onI)
-    apply (rule join_mono[OF compat_jfc' compat_jfc' below_refl cont2monofunE[OF `cont F`]])
-    apply (metis  compatible_F_jfc' fjc'_iff)
-    apply (metis  compatible_F_jfc' fjc'_iff)
-    .
-  next
-  case (goal2 Y)
-    hence "chain Y" by (metis chain_on_is_chain)
-    show ?case
-      apply (rule subst[OF cont2contlubE[OF `cont F` `chain Y`, symmetric]])
-      apply (subst join_cont2[OF ch2ch_cont[OF `cont F` `chain Y`] compatible_F_jfc'[OF chain_on_is_on[OF goal2(1)]]])
-      apply (rule below_refl)
-    done
-  qed
-
-end
-
-lemma subset_fjc': "\<rho> \<sqsubseteq> \<rho>' \<Longrightarrow> fix_join_compat' \<rho>' \<subseteq> fix_join_compat' \<rho>"
-  apply rule
-  apply simp
-  by (rule compatible_down_closed)
-
-lemma fjc'_Inter:
-  assumes "chain Y"
-  shows "(\<Inter> i. (fix_join_compat' (Y i))) = fix_join_compat' (\<Squnion>i. Y i)" (is "?L = ?R")
-proof
-  show "?L \<subseteq> ?R" by (auto intro: admD[OF compatible_adm1 `chain Y`])
-next
-  show "?R \<subseteq> ?L" by (auto elim: compatible_down_closed intro: is_ub_thelub[OF `chain Y`])
-qed
-
-definition fix_join_compat'' where 
-  "fix_join_compat'' (\<rho>::'a::{Bounded_Nonempty_Meet_cpo,subpcpo_partition})  F = {\<rho>'. \<rho>' \<sqsubseteq> fix_on' (to_bot \<rho>) (\<lambda> \<rho>'. \<rho> \<squnion> F \<rho>')}"
-
-lemma fjc''_iff[iff]:
-  "\<rho>' \<in> fix_join_compat'' \<rho> F \<longleftrightarrow> \<rho>' \<sqsubseteq> fix_on' (to_bot \<rho>) (\<lambda> \<rho>'. \<rho> \<squnion> F \<rho>')"
-  unfolding fix_join_compat''_def by auto
-
-lemma subcpo_jfc'': "subcpo (fix_join_compat'' \<rho> F)"
-  unfolding fix_join_compat''_def by (rule subcpo_cone_below)
-
-lemma subpcpo_jfc'': "subpcpo (fix_join_compat'' \<rho> F)"
-  unfolding fix_join_compat''_def by (rule subpcpo_cone_below)
-
-lemma subpcpo_bot_jfc'': "subpcpo_bot (fix_join_compat'' \<rho> F) (to_bot \<rho>)"
-  apply (rule subpcpo_botI)
-  apply (metis subcpo.cpo' subcpo_jfc'')
+  apply (metis subcpo.cpo' subcpo_fjc)
   apply (auto)
   by (metis to_bot_fix_on to_bot_minimal unrelated)
 
-lemma bottom_of_jfc'': "bottom_of (fix_join_compat'' \<rho> F) = to_bot \<rho>"
-  by (rule bottom_of_subpcpo_bot[OF subpcpo_bot_jfc''])
+lemma bottom_of_fjc: "bottom_of (fix_join_compat \<rho> F) = to_bot \<rho>"
+  by (rule bottom_of_subpcpo_bot[OF subpcpo_bot_fjc])
 
-lemma down_closed_jfc'': "down_closed (fix_join_compat'' \<rho> F)"
+lemma down_closed_fjc: "down_closed (fix_join_compat \<rho> F)"
   by (auto intro: down_closedI dest:below_trans)
 
-lemma compat_jfc'': "x \<in> fix_join_compat'' \<rho> F \<Longrightarrow> y \<in> fix_join_compat'' \<rho> F \<Longrightarrow> compatible x y"
+lemma compat_fjc: "x \<in> fix_join_compat \<rho> F \<Longrightarrow> y \<in> fix_join_compat \<rho> F \<Longrightarrow> compatible x y"
   by (auto elim:ub_implies_compatible)
 
-lemma join_jfc'': "x \<in> fix_join_compat'' \<rho> F \<Longrightarrow> y \<in> fix_join_compat'' \<rho> F \<Longrightarrow> x \<squnion> y \<in> fix_join_compat'' \<rho> F"
-  by (rule, metis join_below[OF compat_jfc''] fjc''_iff)
+lemma join_fjc: "x \<in> fix_join_compat \<rho> F \<Longrightarrow> y \<in> fix_join_compat \<rho> F \<Longrightarrow> x \<squnion> y \<in> fix_join_compat \<rho> F"
+  by (rule, metis join_below[OF compat_fjc] fjc_iff)
 
-lemma closed_on_join_jfc'': "closed_on (fix_join_compat'' \<rho> F) G \<Longrightarrow> closed_on (fix_join_compat'' \<rho> F) H \<Longrightarrow> closed_on (fix_join_compat'' \<rho> F) (\<lambda> x. G x \<squnion> H x)"
+lemma closed_on_join_fjc: "closed_on (fix_join_compat \<rho> F) G \<Longrightarrow> closed_on (fix_join_compat \<rho> F) H \<Longrightarrow> closed_on (fix_join_compat \<rho> F) (\<lambda> x. G x \<squnion> H x)"
   apply (rule closed_onI)
-  apply (rule join_jfc'')
+  apply (rule join_fjc)
   apply (erule (1) closed_onE)+
   done
 
-lemma cont_on_join_jfc':
-  assumes "closed_on (fix_join_compat'' \<rho> F) G"
-  assumes "closed_on (fix_join_compat'' \<rho> F) H"
-  assumes "cont_on  (fix_join_compat'' \<rho> F) G"
-  assumes "cont_on  (fix_join_compat'' \<rho> F) H"
-  shows "cont_on (fix_join_compat'' \<rho> F) (\<lambda> x. G x \<squnion> H x)"
-  proof(rule subpcpo.cont_onI2[OF subpcpo_jfc''])
+lemma cont_on_join_fjc:
+  assumes "closed_on (fix_join_compat \<rho> F) G"
+  assumes "closed_on (fix_join_compat \<rho> F) H"
+  assumes "cont_on  (fix_join_compat \<rho> F) G"
+  assumes "cont_on  (fix_join_compat \<rho> F) H"
+  shows "cont_on (fix_join_compat \<rho> F) (\<lambda> x. G x \<squnion> H x)"
+  proof(rule subpcpo.cont_onI2[OF subpcpo_fjc])
   case goal1
   show ?case
     proof(rule monofun_onI)
     case (goal1 x y)
       hence "compatible (G x) (H x)" and "compatible (G y) (H y)"
-        by -(rule compat_jfc''[OF closed_onE[OF assms(1)] closed_onE[OF assms(2)]], assumption+)+
+        by -(rule compat_fjc[OF closed_onE[OF assms(1)] closed_onE[OF assms(2)]], assumption+)+
       moreover
       from goal1
       have "G x \<sqsubseteq> G y"
@@ -162,181 +78,101 @@ lemma cont_on_join_jfc':
       apply (rule join_cont12)
       apply (rule chain_on_is_chain[OF ch2ch_cont_on'[OF assms(3) goal2(1) assms(1)]])
       apply (rule chain_on_is_chain[OF ch2ch_cont_on'[OF assms(4) goal2(1) assms(2)]])
-      apply (rule compat_jfc''[OF closed_onE[OF assms(1) chain_on_is_on[OF goal2(1)]] closed_onE[OF assms(2) chain_on_is_on[OF goal2(1)]]])
+      apply (rule compat_fjc[OF closed_onE[OF assms(1) chain_on_is_on[OF goal2(1)]] closed_onE[OF assms(2) chain_on_is_on[OF goal2(1)]]])
       done
    finally show ?case by (rule eq_imp_below)
 qed
 
-inductive fix_on_cond_jfc'
-  where fix_on_cond_jfc'I:
+subsubsection {* Conditions for the existance of the fixed point of binary joins *}
+
+inductive fix_join_cond
+  where fix_join_condI:
   "cont F \<Longrightarrow>
-   (\<And> i. compatible \<rho> (F (((\<lambda>\<rho>'. \<rho> \<squnion> F \<rho>')^^i) (to_bot \<rho>)))) \<Longrightarrow> fix_on_cond_jfc' \<rho> F "
+   (\<And> i. compatible \<rho> (F (((\<lambda>\<rho>'. \<rho> \<squnion> F \<rho>')^^i) (to_bot \<rho>)))) \<Longrightarrow> fix_join_cond \<rho> F "
 
 
 context
   fixes \<rho> :: "'a::{Bounded_Nonempty_Meet_cpo,subpcpo_partition}" and S and F
-  assumes "fix_on_cond_jfc' \<rho> F"
+  assumes "fix_join_cond \<rho> F"
 begin
-  lemma cont_F_jfc'': "cont F"
-    by (rule fix_on_cond_jfc'.induct[OF `fix_on_cond_jfc' _ _`]) 
+  lemma cont_F_fjc: "cont F"
+    by (rule fix_join_cond.induct[OF `fix_join_cond _ _`]) 
 
-  lemma chain_compat_jfc'': "compatible \<rho> (F (((\<lambda>\<rho>'. \<rho> \<squnion> F \<rho>')^^i) (to_bot \<rho>)))"
-    by (rule fix_on_cond_jfc'.induct[OF `fix_on_cond_jfc' _ _`]) 
+  lemma chain_compat_fjc: "compatible \<rho> (F (((\<lambda>\<rho>'. \<rho> \<squnion> F \<rho>')^^i) (to_bot \<rho>)))"
+    by (rule fix_join_cond.induct[OF `fix_join_cond _ _`]) 
 
-  lemma chain_jfc'': "chain (\<lambda>i. ((\<lambda>\<rho>'. \<rho> \<squnion> F \<rho>')^^i) (to_bot \<rho>))"
+  lemma chain_fjc: "chain (\<lambda>i. ((\<lambda>\<rho>'. \<rho> \<squnion> F \<rho>')^^i) (to_bot \<rho>))"
   proof(rule chainI, induct_tac i, simp_all)
     have "to_bot \<rho> \<sqsubseteq> \<rho>"
       by (rule to_bot_minimal)
     also have "\<rho> \<sqsubseteq> \<rho> \<squnion> F (to_bot \<rho>)"
-      by (rule join_above1[OF chain_compat_jfc''[of 0, simplified]])
+      by (rule join_above1[OF chain_compat_fjc[of 0, simplified]])
     finally
     show "to_bot \<rho> \<sqsubseteq> \<rho> \<squnion> F (to_bot \<rho>)".
    
     fix n
     assume "((\<lambda>\<rho>'. \<rho> \<squnion> F \<rho>') ^^ n) (to_bot \<rho>) \<sqsubseteq> \<rho> \<squnion> F (((\<lambda>\<rho>'. \<rho> \<squnion> F \<rho>') ^^ n) (to_bot \<rho>))"
     thus "\<rho> \<squnion> F (((\<lambda>\<rho>'. \<rho> \<squnion> F \<rho>') ^^ n) (to_bot \<rho>)) \<sqsubseteq> \<rho> \<squnion> F (\<rho> \<squnion> F (((\<lambda>\<rho>'. \<rho> \<squnion> F \<rho>') ^^ n) (to_bot \<rho>)))"
-      by (rule join_mono[OF chain_compat_jfc'' chain_compat_jfc''[of "Suc n", simplified] below_refl cont2monofunE[OF `cont F`]])
+      by (rule join_mono[OF chain_compat_fjc chain_compat_fjc[of "Suc n", simplified] below_refl cont2monofunE[OF `cont F`]])
   qed 
   
-  lemma rho_jfc'': "\<rho> \<in> fix_join_compat'' \<rho> F"
+  lemma rho_fjc: "\<rho> \<in> fix_join_compat \<rho> F"
     apply auto
-    apply (subst fix_on_def, subst if_P[OF chain_jfc''])
-    apply (rule below_trans[OF _ is_ub_thelub[of _ 1, OF chain_jfc'']])
+    apply (subst fix_on_def, subst if_P[OF chain_fjc])
+    apply (rule below_trans[OF _ is_ub_thelub[of _ 1, OF chain_fjc]])
     apply (simp del: funpow.simps(1))
     apply (rule join_above1)
-    apply (rule fix_on_cond_jfc'.induct[OF `fix_on_cond_jfc' _ _`])
+    apply (rule fix_join_cond.induct[OF `fix_join_cond _ _`])
     apply assumption
     done
 
-  lemma F_pres_compat'': "x \<in> fix_join_compat'' \<rho> F \<Longrightarrow> F x \<in> fix_join_compat'' \<rho> F" 
+  lemma F_pres_compat'': "x \<in> fix_join_compat \<rho> F \<Longrightarrow> F x \<in> fix_join_compat \<rho> F" 
     apply auto
-    apply (drule cont2monofunE[OF cont_F_jfc''])
+    apply (drule cont2monofunE[OF cont_F_fjc])
     apply (erule below_trans)
-    apply (subst (1 2) fix_on_def, subst (1 2) if_P[OF chain_jfc''])
-    apply (subst cont2contlubE[OF cont_F_jfc'' chain_jfc''])
-    apply (subst lub_range_shift[symmetric, OF chain_jfc'', of 1])
-    apply (rule lub_mono[OF ch2ch_cont[OF cont_F_jfc'' chain_jfc''] chain_shift[OF chain_jfc'']])
+    apply (subst (1 2) fix_on_def, subst (1 2) if_P[OF chain_fjc])
+    apply (subst cont2contlubE[OF cont_F_fjc chain_fjc])
+    apply (subst lub_range_shift[symmetric, OF chain_fjc, of 1])
+    apply (rule lub_mono[OF ch2ch_cont[OF cont_F_fjc chain_fjc] chain_shift[OF chain_fjc]])
     apply simp
-    apply (rule join_above2[OF chain_compat_jfc''])
+    apply (rule join_above2[OF chain_compat_fjc])
     done
 
-  lemma rho_F_compat_jfc'': "x \<in> fix_join_compat'' \<rho> F \<Longrightarrow> compatible \<rho> (F x)"
-    by (rule compat_jfc''[OF rho_jfc'' F_pres_compat''])
+  lemma rho_F_compat_fjc: "x \<in> fix_join_compat \<rho> F \<Longrightarrow> compatible \<rho> (F x)"
+    by (rule compat_fjc[OF rho_fjc F_pres_compat''])
 
-
-(*
-context
-  fixes \<rho> :: "'a::{Bounded_Nonempty_Meet_cpo,subpcpo_partition}"
-  fixes F :: "'a \<Rightarrow> 'a"
-  assumes "cont F"
-  assumes F_pres_compat: "\<And> x. compatible \<rho> x \<Longrightarrow> compatible \<rho> (F x)"
-begin
-  lemma rho_jfc'': "\<rho> \<in> fix_join_compat'' \<rho> F"
-    apply auto
-    apply (subst fix_on_jfc'_eq[OF `cont F` F_pres_compat], assumption)
-    apply (rule join_above1)
-    apply (metis (full_types) F_pres_compat `cont F`  fjc'_iff subpcpo.fix_on_there[OF subpcpo_jfc' cont_on_jfc' closed_on_jfc'])
-    done    
-
-  lemma F_pres_compat'': "x \<in> fix_join_compat'' \<rho> F \<Longrightarrow> F x \<in> fix_join_compat'' \<rho> F" 
-    apply auto
-    apply (subst fix_on_jfc'_eq[OF `cont F` F_pres_compat], assumption)
-    apply (rule below_trans)
-    apply (erule cont2monofunE[OF `cont F`])
-    apply (rule join_above2)
-    by (metis (full_types) F_pres_compat `cont F` closed_on_jfc' compatible_F_jfc' cont_on_jfc' subpcpo.fix_on_there subpcpo_jfc')
-*)
-
-  lemma F_closed_on_jfc'': "closed_on (fix_join_compat'' \<rho> F) F"
+  lemma F_closed_on_fjc: "closed_on (fix_join_compat \<rho> F) F"
     by (rule, rule F_pres_compat'')
 
-  lemma closed_jfc'': "x \<in> fix_join_compat'' \<rho> F \<Longrightarrow> \<rho> \<squnion> F x \<in> fix_join_compat'' \<rho> F"
-    by (metis F_pres_compat'' rho_jfc'' join_jfc'')
+  lemma closed_fjc: "x \<in> fix_join_compat \<rho> F \<Longrightarrow> \<rho> \<squnion> F x \<in> fix_join_compat \<rho> F"
+    by (metis F_pres_compat'' rho_fjc join_fjc)
 
-  lemma closed_on_jfc'': "closed_on (fix_join_compat'' \<rho> F) (\<lambda> x. \<rho> \<squnion> F x)"
-    by (rule closed_onI, rule closed_jfc'')
+  lemma closed_on_fjc: "closed_on (fix_join_compat \<rho> F) (\<lambda> x. \<rho> \<squnion> F x)"
+    by (rule closed_onI, rule closed_fjc)
 
-  lemma cont_on_jfc'': "cont_on (fix_join_compat'' \<rho> F) (\<lambda> x. \<rho> \<squnion> F x)"
-    by (rule cont_on_join_jfc'[OF const_closed_on[OF rho_jfc''] F_closed_on_jfc'' cont_is_cont_on[OF cont_const] cont_is_cont_on[OF `cont F`]]) 
+  lemma cont_on_fjc: "cont_on (fix_join_compat \<rho> F) (\<lambda> x. \<rho> \<squnion> F x)"
+    by (rule cont_on_join_fjc[OF const_closed_on[OF rho_fjc] F_closed_on_fjc cont_is_cont_on[OF cont_const] cont_is_cont_on[OF `cont F`]]) 
 
-  lemma fix_on_cond_jfc'':
-    "fix_on_cond (fix_join_compat'' \<rho> F) (bottom_of (fix_join_compat'' \<rho> F)) (\<lambda>x. \<rho> \<squnion> F x)"
-    apply (subst bottom_of_jfc'')
-    by (rule fix_on_condI[OF subpcpo_jfc'' bottom_of_jfc'' closed_on_jfc'' cont_on_jfc''])
+  lemma fix_on_cond_fjc:
+    "fix_on_cond (fix_join_compat \<rho> F) (bottom_of (fix_join_compat \<rho> F)) (\<lambda>x. \<rho> \<squnion> F x)"
+    apply (subst bottom_of_fjc)
+    by (rule fix_on_condI[OF subpcpo_fjc bottom_of_fjc closed_on_fjc cont_on_fjc])
 
-  lemma fix_on_jfc''_ind:
-    assumes "adm_on (fix_join_compat'' \<rho> F) P"
-    assumes "P (bottom_of (fix_join_compat'' \<rho> F))"
-    assumes "\<And> y. y \<in> fix_join_compat'' \<rho> F \<Longrightarrow> P y \<Longrightarrow> P (\<rho> \<squnion> F y)"
-    shows "P (fix_on (fix_join_compat'' \<rho> F) (\<lambda> x. \<rho> \<squnion> F x))"
-      by (rule fix_on_ind[OF fix_on_cond_jfc'' assms])
+  lemma fix_on_fjc_ind:
+    assumes "adm_on (fix_join_compat \<rho> F) P"
+    assumes "P (bottom_of (fix_join_compat \<rho> F))"
+    assumes "\<And> y. y \<in> fix_join_compat \<rho> F \<Longrightarrow> P y \<Longrightarrow> P (\<rho> \<squnion> F y)"
+    shows "P (fix_on (fix_join_compat \<rho> F) (\<lambda> x. \<rho> \<squnion> F x))"
+      by (rule fix_on_ind[OF fix_on_cond_fjc assms])
 
-  lemma fix_on_jfc''_eq:
-    shows "fix_on (fix_join_compat'' \<rho> F) (\<lambda> x. \<rho> \<squnion> F x) = \<rho> \<squnion> F (fix_on (fix_join_compat'' \<rho> F) (\<lambda> x. \<rho> \<squnion> F x))"
-    by (rule fix_on_eq[OF fix_on_cond_jfc''])
+  lemma fix_on_fjc_eq:
+    shows "fix_on (fix_join_compat \<rho> F) (\<lambda> x. \<rho> \<squnion> F x) = \<rho> \<squnion> F (fix_on (fix_join_compat \<rho> F) (\<lambda> x. \<rho> \<squnion> F x))"
+    by (rule fix_on_eq[OF fix_on_cond_fjc])
 end
 
-(*
-lemma fix_on_jfc''_mono'':
-  fixes \<rho> \<rho>':: "'a::{Bounded_Nonempty_Meet_cpo, subpcpo_partition}"
-  assumes "\<rho> \<sqsubseteq> \<rho>'"
-  assumes "cont F"
-  assumes F_pres_compat1: "\<And> i x. compatible \<rho> x \<Longrightarrow> compatible \<rho> (F x)"
-  assumes F_pres_compat2: "\<And> i x. compatible \<rho>' x \<Longrightarrow> compatible \<rho>' (F x)"
+subsubsection {* Continutiy of the fixed point of joins *}
 
-  shows "fix_on (fix_join_compat'' \<rho> F) (\<lambda> x. \<rho> \<squnion> F x) \<sqsubseteq> (fix_on (fix_join_compat'' \<rho>' F) (\<lambda> x. \<rho>' \<squnion> F x))"
-  apply (rule parallel_fix_on_ind[OF subpcpo_jfc'' subpcpo_jfc''])
-  apply (rule adm_is_adm_on, simp)
-  apply (metis closed_on_jfc'' assms(2) assms(3))
-  apply (metis cont_on_jfc'' assms(2) assms(3))
-  apply (metis closed_on_jfc'' assms(2) assms(4))
-  apply (metis cont_on_jfc'' assms(2) assms(4))
-  apply (subst (1 2) bottom_of_jfc'')
-  apply (rule eq_imp_below[OF unrelated[OF assms(1)]])
-  by (metis F_pres_compat1 F_pres_compat2 assms(1) assms(2) cont2monofunE compat_jfc'' rho_jfc'' join_mono)
-*)
-
-lemma subset_fjc'':
-  assumes "cont F"
-  assumes "fix_on_cond_jfc' \<rho> F"
-  assumes "fix_on_cond_jfc' \<rho>' F"
-  shows "\<rho> \<sqsubseteq> \<rho>' \<Longrightarrow> fix_join_compat'' \<rho> F \<subseteq> fix_join_compat'' \<rho>' F"
-  apply rule
-  apply (simp only: fjc''_iff)
-  apply (erule below_trans)
-  apply (rule fix_on_mono2[OF fix_on_cond_jfc''[OF assms(2)] fix_on_cond_jfc''[OF assms(3)], unfolded bottom_of_jfc''])
-  apply (metis po_eq_conv unrelated)
-  by (rule join_mono[OF
-        rho_F_compat_jfc''[OF assms(2)]
-        rho_F_compat_jfc''[OF assms(3)]
-        _
-        cont2monofunE[OF `cont F`]])
-
-(*
-lemma subset_fjc'':
-  assumes "cont F"
-  assumes F_pres_compat1: "\<And> x. compatible \<rho> x \<Longrightarrow> compatible \<rho> (F x)"
-  assumes F_pres_compat2: "\<And> x. compatible \<rho>' x \<Longrightarrow> compatible \<rho>' (F x)"
-  shows "\<rho> \<sqsubseteq> \<rho>' \<Longrightarrow> fix_join_compat'' \<rho> F \<subseteq> fix_join_compat'' \<rho>' F"
-  apply rule
-  apply simp
-  apply (erule below_trans)
-  apply (rule fix_on_mono2[OF subpcpo_jfc' subpcpo_jfc' closed_on_jfc' cont_on_jfc' closed_on_jfc' cont_on_jfc'])
-  apply (auto simp add: assms)
-  apply (metis bottom_of_jfc' po_eq_conv unrelated)
-  apply (erule (3) join_mono[OF F_pres_compat1 F_pres_compat2 _ cont2monofunE[OF `cont F`]])
-  done
-*)
-
-(* Wrong 
-lemma jfc''_Union:
-  assumes "chain Y"
-  assumes "cont F"
-  assumes F_pres_compat: "\<And> i x. compatible (Y i) x \<Longrightarrow> compatible (Y i) (F x)"
-  assumes F_pres_compat': "\<And> x. compatible (\<Squnion> i. Y i) x \<Longrightarrow> compatible (\<Squnion> i. Y i) (F x)"
-*)
-
-lemma fix_on_join_cont'_general:
+lemma fix_on_join_cont_general:
   fixes F :: "'a::Bounded_Nonempty_Meet_cpo \<Rightarrow> 'a"
   assumes "subpcpo S'"
   assumes pcpo_i: "\<And> i. subpcpo (S i)"
@@ -477,241 +313,44 @@ proof-
   show ?thesis.
 qed
 
-
-lemma fix_on_join_cont':
-  fixes F :: "'a::Bounded_Nonempty_Meet_cpo \<Rightarrow> 'a"
-  assumes pcpo_i: "\<And> i. subpcpo (S i)"
-  assumes down_closed: "\<And> i. down_closed (S i)"
-  assumes ss: "\<And> i j. S (j + i) \<subseteq> S i"
-  assumes "chain Y"
-  assumes "cont F"
-  assumes compat: "\<And> i x. x \<in> S i \<Longrightarrow> compatible (Y i) (F x)"
-  assumes cl: "\<And> i. closed_on (S i) (\<lambda>x. Y i \<squnion> F x)"
-
-  shows "fix_on (\<Inter> i. S i) (\<lambda> x. (\<Squnion>i. Y i) \<squnion> F x) = (\<Squnion> i. (fix_on (S i) (\<lambda> x. Y i \<squnion> F x)))"
-    (is "fix_on ?S _ = Lub ?F")
-proof(rule fix_on_join_cont'_general[OF _ pcpo_i _ down_closed _ _ `chain Y` `cont F` compat _ cl])
-  show same_bottoms: "\<And> i j. bottom_of (S i) = bottom_of (S j)"
-  proof-
-    {
-    fix i j :: nat
-    assume "i < j"
-    
-    have "S j \<subseteq> S i"
-      using `i < j` by (metis less_imp_add_positive nat_add_commute ss)
-    hence "bottom_of (S j) \<in> S i"
-      by (rule subsetD[OF _ subpcpo.bottom_of_there[OF pcpo_i]])
-    hence b: "bottom_of (S i) \<sqsubseteq> bottom_of (S j)"
-      by (rule subpcpo.bottom_of_minimal[OF pcpo_i])
-    moreover
-    have "bottom_of (S i) \<in> S j"
-      by (rule down_closed.down_closedE[OF down_closed subpcpo.bottom_of_there[OF pcpo_i] b])
-    hence "bottom_of (S j) \<sqsubseteq> bottom_of (S i)"
-      by (rule subpcpo.bottom_of_minimal[OF pcpo_i])
-    finally
-    have "bottom_of (S j) = bottom_of (S i)"..
-    }
-    thus "\<And> i j. bottom_of (S i) = bottom_of (S j)" by (metis linorder_neqE_nat)
-  qed
-
-  interpret subpcpo ?S by (rule subpcpo_Inter[OF pcpo_i same_bottoms])
-  show "subpcpo ?S" by (rule subpcpo_axioms)
-  interpret down_closed ?S by (metis down_closed down_closed_Inter)
-  show "down_closed ?S" by (rule down_closed_axioms)
-
-  show same_bottoms'[simp]: "\<And> i. bottom_of (S i) = bottom_of ?S"
-    by (metis bottom_of_Inter pcpo_i same_bottoms)
-  have ss': "\<And> i. ?S \<subseteq> S i"
-    by (metis INF_lower UNIV_I)
-
-  show compat': "\<And> x. x \<in> ?S \<Longrightarrow> compatible (\<Squnion>i. Y i) (F x)"
-    by (rule admD[OF compatible_adm1 `chain Y` compat[OF subsetD[OF ss']]])
-
-  show cl': "closed_on ?S (\<lambda>x. (\<Squnion> i. Y i) \<squnion> F x)"
-  proof (rule closed_onI)
-    fix x
-    assume  "x \<in> (\<Inter>i. S i)"
-    hence x: "\<And>i. x \<in> S i" by (metis INT_E UNIV_I)
-    have "\<And> i. (\<Squnion> i. Y i) \<squnion> F x \<in> S i"
-    proof-
-      fix i
-      have "chain_on (S i) (\<lambda> j. Y (j + i) \<squnion> F x )"
-        apply (rule chain_onI[OF 
-            join_mono[OF
-               compat[OF x]
-               compat[OF x]
-               _
-               below_refl]
-            subsetD[OF ss closed_onE[OF cl x]]
-            ])
-        by (simp add: chainE[OF `chain Y`])
-      hence "(\<Squnion> j. Y (j + i) \<squnion> F x) \<in> S i" by (rule subpcpo.chain_on_lub_on[OF pcpo_i])
-      hence "(\<Squnion> j. Y (j + i)) \<squnion> F x \<in> S i"
-        by (subst join_cont1[OF chain_shift[OF `chain Y`] compat[OF x]])
-      thus "(\<Squnion> i. Y i) \<squnion> F x \<in> S i"
-        by (subst (asm) lub_range_shift[OF `chain Y`])
-    qed
-    thus "(\<Squnion> i. Y i) \<squnion> F x \<in> (\<Inter>i. S i)" by (metis INT_iff)
-  qed
-qed
-
-lemma closed_on_Union:
-  assumes "\<And> i. closed_on (S i) F"
-  shows "closed_on (\<Union>i. S i) F"
-  apply (rule closed_onI)
-  apply (erule UN_E)
-  apply (rule UN_I[OF UNIV_I])
-  apply (erule closed_onE[OF assms])
-  done
-
-
-lemma fix_on_join_cont'_covariant:
-  fixes F :: "'a::Bounded_Nonempty_Meet_cpo \<Rightarrow> 'a"
-  assumes pcpo: "subpcpo (\<Union> i. S i)"
-  assumes pcpo_i: "\<And> i. subpcpo (S i)"
-  assumes down_closed: "\<And> i. down_closed (S i)"
-  assumes ss: "\<And> i j. S i \<subseteq> S (j + i)"
-  assumes "chain Y"
-  assumes "cont F"
-  assumes compat: "\<And> i x. x \<in> S i \<Longrightarrow> compatible (Y i) (F x)"
-  assumes cl: "\<And> i. closed_on (S i) (\<lambda>x. Y i \<squnion> F x)"
-
-  shows "fix_on (\<Union> i. S i) (\<lambda> x. (\<Squnion>i. Y i) \<squnion> F x) = (\<Squnion> i. (fix_on (S i) (\<lambda> x. Y i \<squnion> F x)))"
-    (is "fix_on ?S _ = Lub ?F")
-proof(rule fix_on_join_cont'_general[OF pcpo pcpo_i _ down_closed _ _ `chain Y` `cont F` compat _ cl])
-  show same_bottoms: "\<And> i j. bottom_of (S i) = bottom_of (S j)"
-  proof-
-    {
-    fix i j :: nat
-    assume "i < j"
-    
-    have "S i \<subseteq> S j"
-      using `i < j` by (metis less_imp_add_positive nat_add_commute ss)
-    hence "bottom_of (S i) \<in> S j"
-      by (rule subsetD[OF _ subpcpo.bottom_of_there[OF pcpo_i]])
-    hence b: "bottom_of (S j) \<sqsubseteq> bottom_of (S i)"
-      by (rule subpcpo.bottom_of_minimal[OF pcpo_i])
-    moreover
-    have "bottom_of (S j) \<in> S i"
-      by (rule down_closed.down_closedE[OF down_closed subpcpo.bottom_of_there[OF pcpo_i] b])
-    hence "bottom_of (S i) \<sqsubseteq> bottom_of (S j)"
-      by (rule subpcpo.bottom_of_minimal[OF pcpo_i])
-    finally
-    have "bottom_of (S i) = bottom_of (S j)"..
-    }
-    thus "\<And> i j. bottom_of (S i) = bottom_of (S j)" by (metis linorder_neqE_nat)
-  qed
-
-  interpret subpcpo ?S by fact
-  interpret down_closed ?S
-    apply (rule down_closedI)
-    apply (erule UN_E)
-    apply (rule UN_I[OF UNIV_I down_closed.down_closedE])
-    by (metis down_closed )
-  show "down_closed ?S" by (rule down_closed_axioms)
-
-  have ss': "\<And> i. S i \<subseteq> ?S"
-    by (metis SUP_upper UNIV_I)
-  show same_bottoms'[simp]: "\<And> i. bottom_of (S i) = bottom_of ?S"
-    apply (rule below_antisym)
-    apply (metis UN_E bottom_of_there pcpo_i same_bottoms subpcpo.bottom_of_minimal)
-    by (metis bottom_of_minimal pcpo_i set_mp ss' subpcpo.bottom_of_there)
-
-  show compat': "\<And> x. x \<in> ?S \<Longrightarrow> compatible (\<Squnion>i. Y i) (F x)"
-  proof-
-    fix x
-    assume "x \<in> ?S"
-    then obtain i where "x \<in> S i" by auto
-    hence "\<And> j. x \<in> S (j + i)" by (metis in_mono ss)
-    hence "\<And> j. compatible (Y (j + i)) (F x)" by (rule compat)
-    hence "compatible (\<Squnion> j. (Y (j + i))) (F x)"
-      by (rule admD[OF compatible_adm1 chain_shift[OF `chain Y`]])
-    thus "compatible (\<Squnion>i. Y i) (F x)"
-      by (metis lub_range_shift[OF `chain Y`])
-  qed
-
-  show cl': "closed_on ?S (\<lambda>x. (\<Squnion> i. Y i) \<squnion> F x)"
-  proof (rule closed_onI)
-    fix x
-    assume  "x \<in> (\<Union>i. S i)"
-    then obtain i where "x \<in> S i" by auto
-    hence j: "\<And> j. x \<in> S (j + i)" by (metis in_mono ss)
-    hence "\<And> j. Y (j + i) \<squnion> (F x) \<in> S (j + i)" by (rule closed_onE[OF cl])
-    hence "\<And> j. Y (j + i) \<squnion> (F x) \<in> (\<Union> i. S i)" by (metis UNIV_I UN_iff)
-    hence "chain_on ?S (\<lambda>j. Y (j + i) \<squnion> (F x))"
-      apply -
-      apply (rule chain_onI)
-      apply (rule join_mono[OF compat[OF j] compat[OF j] _ below_refl])
-      apply (metis add_Suc_right add_Suc_shift chainE[OF `chain Y`])
-      apply assumption
-      done
-    hence "(\<Squnion>j. Y (j + i) \<squnion> (F x)) \<in> (\<Union> i. S i)" by (rule chain_on_lub_on)
-    hence "(\<Squnion>j. Y (j + i)) \<squnion> (F x) \<in> (\<Union> i. S i)"
-      apply (subst join_cont1[OF chain_shift[OF `chain Y`]])
-      apply (rule compat[OF j])
-      apply auto
-      done
-    thus "(\<Squnion>i. Y i) \<squnion> (F x) \<in> (\<Union> i. S i)"
-      by (metis lub_range_shift[OF `chain Y`])
-   qed
-qed
-
-lemma fix_on_join_cont'':
+lemma fix_on_join_cont:
   fixes Y :: "nat \<Rightarrow> 'a::{Bounded_Nonempty_Meet_cpo, subpcpo_partition}"
   assumes "chain Y"
-  assumes "cont F"
-  assumes F_pres_compat: "\<And> i x. compatible (Y i) x \<Longrightarrow> compatible (Y i) (F x)"
+  assumes focj: "\<And>i. fix_join_cond (Y i) F"
+  assumes focj': "fix_join_cond (\<Squnion> i. Y i) F"
 
-  shows "fix_on (fix_join_compat' (\<Squnion> i. Y i)) (\<lambda> x. (\<Squnion>i. Y i) \<squnion> F x) = (\<Squnion> i. (fix_on (fix_join_compat' (Y i)) (\<lambda> x. Y i \<squnion> F x)))"
-proof-
-  have "fix_on (\<Inter> i. (fix_join_compat' (Y i))) (\<lambda> x. (\<Squnion>i. Y i) \<squnion> F x) = (\<Squnion> i. (fix_on (fix_join_compat' (Y i)) (\<lambda> x. Y i \<squnion> F x)))"
-  apply (rule fix_on_join_cont'[OF subpcpo_jfc' down_closed_jfc'])
-  apply (metis subset_fjc'[OF chain_mono[OF `chain Y`]] le_add1 nat_add_commute)
-  apply fact+
-  apply (metis compatible_F_jfc' assms(2) assms(3))
-  apply (metis closed_onI closed_jfc' assms(2) assms(3))
-  done
-  thus ?thesis unfolding fjc'_Inter[OF `chain Y`].
-qed
-
-lemma fix_on_join_cont''':
-  fixes Y :: "nat \<Rightarrow> 'a::{Bounded_Nonempty_Meet_cpo, subpcpo_partition}"
-  assumes "chain Y"
-  assumes focj: "\<And>i. fix_on_cond_jfc' (Y i) F"
-  assumes focj': "fix_on_cond_jfc' (\<Squnion> i. Y i) F"
-
-  shows "fix_on (fix_join_compat'' (\<Squnion> i. Y i) F) (\<lambda> x. (\<Squnion>i. Y i) \<squnion> F x) = (\<Squnion> i. (fix_on (fix_join_compat'' (Y i) F) (\<lambda> x. Y i \<squnion> F x)))"
-proof(rule fix_on_join_cont'_general)
+  shows "fix_on (fix_join_compat (\<Squnion> i. Y i) F) (\<lambda> x. (\<Squnion>i. Y i) \<squnion> F x) = (\<Squnion> i. (fix_on (fix_join_compat (Y i) F) (\<lambda> x. Y i \<squnion> F x)))"
+proof(rule fix_on_join_cont_general)
   fix i
-  show "\<And> j. bottom_of (fix_join_compat'' (Y i) F) = bottom_of (fix_join_compat'' (Y j) F)"
-    apply (simp add: bottom_of_jfc'')
+  show "\<And> j. bottom_of (fix_join_compat (Y i) F) = bottom_of (fix_join_compat (Y j) F)"
+    apply (simp add: bottom_of_fjc)
     by (metis linorder_linear unrelated[OF chain_mono[OF `chain Y`]])
   next
   fix i
-  show "bottom_of (fix_join_compat'' (Y i) F) = bottom_of (fix_join_compat'' (\<Squnion> i. Y i) F)"
-    apply (simp add: bottom_of_jfc'')
+  show "bottom_of (fix_join_compat (Y i) F) = bottom_of (fix_join_compat (\<Squnion> i. Y i) F)"
+    apply (simp add: bottom_of_fjc)
     by (rule unrelated[OF is_ub_thelub[OF `chain Y`]])
   next
   show "cont F"
-    by (rule cont_F_jfc''[OF focj])
+    by (rule cont_F_fjc[OF focj])
   next
   fix i x
-  assume "x \<in> fix_join_compat'' (Y i) F"
+  assume "x \<in> fix_join_compat (Y i) F"
   thus "compatible (Y i) (F x)"
-    by (rule rho_F_compat_jfc''[OF focj])
+    by (rule rho_F_compat_fjc[OF focj])
   next
   fix x
-  assume "x \<in> fix_join_compat'' (\<Squnion> i. Y i) F"
+  assume "x \<in> fix_join_compat (\<Squnion> i. Y i) F"
   thus "compatible (\<Squnion> i. Y i) (F x)"
-    by (rule rho_F_compat_jfc''[OF focj'])
+    by (rule rho_F_compat_fjc[OF focj'])
   next
   fix i
-  show "closed_on (fix_join_compat'' (Y i) F) (\<lambda>x. Y i \<squnion> F x)"
-    by (rule closed_on_jfc''[OF focj])
+  show "closed_on (fix_join_compat (Y i) F) (\<lambda>x. Y i \<squnion> F x)"
+    by (rule closed_on_fjc[OF focj])
   next
   fix i
-  show "closed_on (fix_join_compat'' (\<Squnion> i. Y i) F) (\<lambda>x. (\<Squnion> i. Y i) \<squnion> F x)"
-    by (rule closed_on_jfc''[OF focj'])
-qed (intro subpcpo_jfc'' down_closed_jfc'' rho_F_compat_jfc'' closed_on_jfc'' assms)+
+  show "closed_on (fix_join_compat (\<Squnion> i. Y i) F) (\<lambda>x. (\<Squnion> i. Y i) \<squnion> F x)"
+    by (rule closed_on_fjc[OF focj'])
+qed (intro subpcpo_fjc down_closed_fjc rho_F_compat_fjc closed_on_fjc assms)+
 
 end
